edited the spec of tables + proved property 1

hol/tables_specScript.sml
@@ -100,19 +100,12 @@ End
 
 
 Definition fv_atom_def:
-  fv_atom (Var x) = [x] ∧
+  fv_atom ((Var x):atom_var) = [x] ∧
   fv_atom True = [] ∧
   fv_atom False = [] ∧
-  fv_atom (Not p) = fv_pred p
+  fv_atom (Not p) = fv_atom p
 End
 
-        
-Definition fv_atom_def:
-  fv_atom (Var x) = [x] ∧
-  fv_atom True = [] ∧
-  fv_atom False = [] ∧
-  fv_atom (Not p) = fv_atom p 
-End
                         
                 
 (***************************************************)
@@ -171,10 +164,10 @@ Definition match_tbll_def:
 End
 
  
-(* Top-level table semantics *)       
-Definition sem_tbll_def:
-  sem_tbll (tbll: 'a table_list) mv =
-   match_tbll tbll mv 0
+(* Top-level table semantics, return the starting state as well*)       
+Definition sem_tables_def:
+  sem_tables ((tbll: 'a table_list),st_in) mv =
+   match_tbll tbll mv st_in
 End
 
 
@@ -200,7 +193,10 @@ Definition mk_substitute_tbll_def:
 End
 
 
-
+Definition mk_substitute_tables_def:
+  mk_substitute_tables ((tbll: 'a table_list), st_in) x b =
+   (mk_substitute_tbll tbll x b, st_in:num)
+End
         
 (* table simplifications *)
 
@@ -222,7 +218,10 @@ Definition simp_tbll_def:
 End
 
 
-
+Definition simp_tables_def:
+  simp_tables ((tbll: 'a table_list), st_in) =
+   (simp_tbll tbll, st_in:num)
+End
 
 (* table final *)
 
@@ -280,11 +279,9 @@ End
 
 
 
-
-        
-Definition final_tbll_ete_def:
-  final_tbll_ete tbll =
-  final_tbll tbll 0
+Definition final_tables_def:
+  final_tables (tbll, st_in) =
+  final_tbll tbll st_in
 End
 
         
@@ -300,13 +297,12 @@ Definition fv_row_def:
 End
 
 
-
 Definition fv_tbl_def:
   fv_tbl (tbl: 'a table) =
-  let fv_in_tbl = MAP (\(atoml, st_num, res). fv_row atoml) tbl in
-    nub(FLAT fv_in_tbl)
+  (let fv_in_tbl = MAP(\(atom,st_num,res). fv_row atom) tbl in
+      nub (FLAT fv_in_tbl))
 End
-
+        
         
 
     
@@ -316,29 +312,566 @@ Definition fv_tbll_def:
     nub(FLAT fv_in_tbll)
 End
 
+
+        
+Definition fv_tables_def:
+  fv_tables (tbll, st_in) =
+  fv_tbll tbll
+End
+
+
+
+        
                                                                  
 Definition table_structure_def:
   table_structure =
   <|
-    sem := sem_tbll;
-    sub := mk_substitute_tbll;
-    simp := simp_tbll;
-    final := final_tbll_ete;
-    fv := fv_tbll;
+    sem := sem_tables;
+    sub := mk_substitute_tables;
+    simp := simp_tables;
+    final := final_tables;
+    fv := fv_tables;
   |>
 End            
 
-               
 
-Theorem fv_mem_table_thm:
-  ∀ h p mv.
-    (∀x. MEM x (fv_tbll (h::p)) ⇒ ∃b. ALOOKUP mv x = SOME b) ⇒
-    (∀x. MEM x (fv_tbll p) ⇒ ∃b. ALOOKUP mv x = SOME b)
+
+               
+Theorem fv_mem_tbll_thm:
+  ∀ tbll tbl mv.
+    (∀x. MEM x (fv_tbll (tbl::tbll)) ⇒ ∃b. ALOOKUP mv x = SOME b) ⇒
+    (∀x. MEM x (fv_tbll  tbll) ⇒ ∃b. ALOOKUP mv x = SOME b)
 Proof
-  gvs[fv_tbll_def]  
+  gvs[fv_tbll_def]
 QED
 
+        
+Theorem fv_mem_tbll_hd_thm:
+  ∀ tbll tbl mv.
+    (∀x. MEM x (fv_tbll (tbl::tbll)) ⇒ ∃b. ALOOKUP mv x = SOME b) ⇒
+    (∀x. MEM x (fv_tbl  tbl) ⇒ ∃b. ALOOKUP mv x = SOME b)
+Proof
+  gvs[fv_tbll_def, fv_tbl_def]
+QED
+        
+
+Theorem fv_mem_tbl_thm:
+  ∀ tbl h mv.
+    (∀x. MEM x (fv_tbl (h::tbl)) ⇒ ∃b. ALOOKUP mv x = SOME b) ⇒
+    (∀x. MEM x (fv_tbl  tbl) ⇒ ∃b. ALOOKUP mv x = SOME b)
+Proof
+  gvs[fv_tbl_def]
+QED
+
+
+Theorem fv_mem_tbl_h_thm:
+  ∀ tbl h mv.
+    (∀x. MEM x (fv_tbl (h::tbl)) ⇒ ∃b. ALOOKUP mv x = SOME b) ⇒
+    (∀x. MEM x (fv_tbl  [h]) ⇒ ∃b. ALOOKUP mv x = SOME b)
+Proof
+  gvs[fv_tbl_def]
+QED        
+
+
+
+Theorem fv_mem_row_thm:
+  ∀ atoml h mv.
+    (∀x. MEM x (fv_row (h::atoml)) ⇒ ∃b. ALOOKUP mv x = SOME b) ⇒
+    (∀x. MEM x (fv_row atoml) ⇒ ∃b. ALOOKUP mv x = SOME b)
+Proof
+  gvs[fv_row_def]
+QED 
+
+
+
+Theorem fv_mem_row_h_thm:
+  ∀ atoml h mv.
+    (∀x. MEM x (fv_row (h::atoml)) ⇒ ∃b. ALOOKUP mv x = SOME b) ⇒
+    (∀x. MEM x (fv_row [h]) ⇒ ∃b. ALOOKUP mv x = SOME b)
+Proof
+  gvs[fv_row_def]
+QED
+
+
+Theorem fv_mem_atom_not_thm:        
+  ∀ atom mv.
+    (∀x. MEM x (fv_row [Not atom]) ⇒ ∃b. ALOOKUP mv x = SOME b) ⇒
+    (∀x. MEM x (fv_row [atom]) ⇒ ∃b. ALOOKUP mv x = SOME b)
+Proof     
+  gvs[fv_row_def, fv_atom_def]
+QED
+
+
+          
+Theorem mk_substitute_tbl_normalize1:
+  ∀h rows x b.
+       mk_substitute_tbl (h::rows) x b =
+       mk_substitute_tbl [h] x b ⧺ mk_substitute_tbl rows x b
+Proof
+  gvs[mk_substitute_tbl_def]
+QED
+
+
+Theorem mk_substitute_tbl_normalize2:
+  ∀atoml st_num res rows x b.
+       mk_substitute_tbl ((atoml,st_num,res)::rows) x b =
+       (mk_substitute_row atoml x b,st_num,res)::mk_substitute_tbl rows x b
+Proof
+  gvs[mk_substitute_tbl_def]
+QED
+
+
+Theorem simp_tbl_normalize1:
+  ∀atoml st_num res rows x b.
+       simp_tbl ((atoml,st_num,res)::rows) =
+       (simp_row atoml,st_num,res)::simp_tbl rows
+Proof
+  gvs[simp_tbl_def]
+QED
+
+
+        
+Theorem sub_then_simp_answer_indeed_in_fv:
+  ∀ atom h' b s.                      
+    (simp_atom (mk_substitute_atom atom h' b) = Var s) ⇒
+    MEM s (fv_atom atom)
+Proof
+  Induct >>
+  rpt strip_tac >>
+  gvs[fv_atom_def, mk_substitute_atom_def, simp_atom_def] >>
+  rpt (BasicProvers.FULL_CASE_TAC >> gvs[]) >>
+  gvs[fv_atom_def, mk_substitute_atom_def, simp_atom_def] 
+QED
+
+
+Triviality simp_fv_not_triv1:
+  ∀ atom h' b x a.
+    simp_atom (mk_substitute_atom atom h' b) = Not a ∧
+    MEM x (fv_atom a) ⇒
+    MEM x (fv_atom (simp_atom (mk_substitute_atom atom h' b)))
+Proof
+  gvs[fv_atom_def, mk_substitute_atom_def, simp_atom_def] 
+QED
+        
+
+Triviality mem_fv_sub_simp_tbl_triv1:
+  ∀ atom h' b x.        
+    MEM x (fv_atom (simp_atom (mk_substitute_atom atom h' b))) ⇒
+    MEM x (fv_atom atom)
+Proof
+  Induct >>
+  rpt strip_tac >>
+  gvs[fv_atom_def, mk_substitute_atom_def, simp_atom_def] >>
+  rpt (BasicProvers.FULL_CASE_TAC >> gvs[]) >>
+  gvs[fv_atom_def, mk_substitute_atom_def, simp_atom_def] >>
+  imp_res_tac sub_then_simp_answer_indeed_in_fv >>
+  imp_res_tac simp_fv_not_triv1 >>
+  res_tac 
+QED
              
+
+Theorem sub_then_simp_not_answer_indeed_in_fv:
+  ∀ atom atom' h' b mv.                      
+    (∀x. MEM x (fv_atom atom) ⇒ ∃b. ALOOKUP mv x = SOME b) ∧
+    simp_atom (mk_substitute_atom atom h' b) = Not atom'
+    ⇒
+    (∀x. MEM x (fv_atom atom') ⇒ ∃b. ALOOKUP mv x = SOME b)
+Proof
+  Induct >>
+  rpt strip_tac >>
+  gvs[fv_atom_def, mk_substitute_atom_def, simp_atom_def] >>
+  rpt (BasicProvers.FULL_CASE_TAC >> gvs[]) >>
+  gvs[fv_atom_def, mk_substitute_atom_def, simp_atom_def] >>
+  assume_tac sub_then_simp_answer_indeed_in_fv >>
+  first_x_assum (strip_assume_tac o (Q.SPECL [‘atom’, ‘h'’, ‘b’, ‘s’])) >>
+  gvs[] >>
+  imp_res_tac mem_fv_sub_simp_tbl_triv1 >> res_tac >> gvs[]
+QED
+      
+
+Theorem mem_imp_sem_tbl:
+  ∀ atom mv.
+    (∀x. MEM x (fv_atom atom) ⇒ ∃b. ALOOKUP mv x = SOME b) ⇒
+    sem_atom atom mv ≠ NONE ∧ ∃ b' . sem_atom atom mv = SOME b'
+Proof
+  Induct >>
+  rw[fv_atom_def] >> gvs[AllCaseEqs()] >>
+  gvs[sem_atom_def, simp_atom_def] >>
+  rpt (BasicProvers.FULL_CASE_TAC >> gvs[]) 
+QED
+
+
+Triviality non_empty_line_simp_not_empty:
+  ∀ atoml h' b.
+    atoml ≠ [] ⇔  simp_row (mk_substitute_row atoml h' b) ≠ []
+Proof
+  Induct >> gvs[mk_substitute_row_def, simp_row_def]
+QED
+
+
+
+Theorem lookup_implies_sem_atoms_same:
+  ∀ atom h' b bool mv.
+    ALOOKUP mv h' = SOME b  ⇒
+    (sem_atom atom mv = SOME bool ⇔
+       sem_atom (simp_atom (mk_substitute_atom atom h' b)) mv = SOME bool)
+Proof
+  Induct >>
+  rpt strip_tac >>
+  rpt (gvs[mk_substitute_atom_def, simp_atom_def, sem_atom_def] >>
+       BasicProvers.FULL_CASE_TAC >>
+       res_tac >>               
+       gvs[]) >>
+  gvs[mk_substitute_atom_def, simp_atom_def, sem_atom_def] >>
+  metis_tac[]
+QED
+           
+
+Theorem lookup_implies_sem_atoml_same1:
+  ∀ atoml h' b mv.
+    ALOOKUP mv h' = SOME b ∧
+    EVERY (λminipred. sem_atom minipred mv = SOME T) atoml ⇒
+    EVERY ((λminipred. sem_atom minipred mv = SOME T)) (simp_row (mk_substitute_row atoml h' b))
+Proof
+  Induct >>
+  rpt strip_tac >>            
+  gvs[mk_substitute_row_def, simp_row_def] >>
+  imp_res_tac lookup_implies_sem_atoms_same
+QED
+
+
+Theorem lookup_implies_sem_atoml_same2:
+  ∀ atoml h' b mv.
+    ALOOKUP mv h' = SOME b ∧
+    EVERY ((λminipred. sem_atom minipred mv = SOME T)) (simp_row (mk_substitute_row atoml h' b)) ⇒
+    EVERY (λminipred. sem_atom minipred mv = SOME T) atoml
+Proof
+  Induct >>
+  rpt strip_tac >> 
+  gvs[mk_substitute_row_def, simp_row_def] >>
+  imp_res_tac lookup_implies_sem_atoms_same >> gvs[] >> res_tac 
+QED
+
+
+         
+Theorem  sem_hd_line_imp_is_match_row:
+  ∀ atoml st_num res h' b s_in mv.
+    ALOOKUP mv h' = SOME b ∧
+    sem_tables ([simp_tbl (mk_substitute_tbl [(atoml,st_num,res)] h' b)],s_in) mv =
+    sem_tables ([[(atoml,st_num,res)]],s_in) mv  ⇒
+    is_match_row s_in st_num atoml mv =
+    is_match_row s_in st_num (simp_row (mk_substitute_row atoml h' b)) mv
+Proof
+  rpt strip_tac >>
+  gvs[sem_tables_def, match_tbll_def] >>
+  
+  Cases_on ‘match_tbl (simp_tbl (mk_substitute_tbl [(atoml,st_num,res)] h' b)) mv s_in’ >>
+  gvs[] >>
+  Cases_on ‘match_tbl [(atoml,st_num,res)] mv s_in’ >>
+  gvs[] >>
+  
+  
+  (gvs[match_tbl_def, min_idx_till_def] >>
+   rpt (BasicProvers.FULL_CASE_TAC >> gvs[]) >> 
+   gvs[check_all_rows_match_def] >>
+                    
+   imp_res_tac INDEX_FIND_NONE_EXISTS >>
+   gvs[] >>
+   gvs[mk_substitute_tbl_def, simp_tbl_def] >>
+   
+   imp_res_tac P_holds_on_curent >>
+   PairCases_on ‘r’ >>
+   gvs[]) >>
+  
+  
+  gvs[is_match_row_def] >>
+  rpt strip_tac >>
+  gvs[is_atoml_true_def] >>
+  gvs[INDEX_FIND_EQ_SOME_0] >>
+  gvs[is_match_row_def] >>
+  gvs[is_atoml_true_def] >|[
+    
+    imp_res_tac lookup_implies_sem_atoml_same1 >> gvs[] >>
+    imp_res_tac NOT_EVERY
+    ,
+    imp_res_tac non_empty_line_simp_not_empty
+    ,
+    
+    imp_res_tac lookup_implies_sem_atoml_same2 >> gvs[] >>
+    imp_res_tac NOT_EVERY
+    ,
+    
+    imp_res_tac non_empty_line_simp_not_empty >> gvs[]
+  ]
+QED
+
+
+
+Theorem is_match_row_substitute_preserve1:
+  ∀ atoml mv h' b s_in st_num.        
+    ALOOKUP mv h' = SOME b ∧
+    is_match_row s_in st_num atoml mv ⇒
+    is_match_row s_in st_num (simp_row (mk_substitute_row atoml h' b)) mv
+Proof
+  Induct >>
+  gvs[is_match_row_def] >>
+  rpt strip_tac >>
+  gvs[is_atoml_true_def] >>
+  (
+  imp_res_tac lookup_implies_sem_atoml_same1 >> gvs[] >>
+  gvs[mk_substitute_row_def, simp_row_def] >>
+  imp_res_tac lookup_implies_sem_atoms_same
+  )
+QED
+
+
+
+Theorem is_match_row_substitute_preserve2:
+  ∀ atoml mv h' b s_in st_num.        
+    ALOOKUP mv h' = SOME b ∧
+    is_match_row s_in st_num (simp_row (mk_substitute_row atoml h' b)) mv ⇒
+    is_match_row s_in st_num atoml mv
+Proof
+  Induct >>
+  gvs[is_match_row_def] >>
+  rpt strip_tac >>
+  gvs[is_atoml_true_def] >>
+  (
+  imp_res_tac lookup_implies_sem_atoml_same2 >> 
+  gvs[mk_substitute_row_def, simp_row_def] 
+  )
+QED
+
+
+
+Theorem is_match_row_substitute_preserve:
+  ∀ atoml mv h' b (s_in:num) st_num.        
+    ALOOKUP mv h' = SOME b ⇒
+    (is_match_row s_in st_num (simp_row (mk_substitute_row atoml h' b)) mv =
+    is_match_row s_in st_num atoml mv)
+Proof
+  rpt strip_tac >>
+  EQ_TAC >>
+  metis_tac[is_match_row_substitute_preserve1, is_match_row_substitute_preserve2]
+QED
+
+
+
+Theorem exists_is_match_row_after_subst_simp:        
+  ∀ tbl s_in h' b mv.
+    ALOOKUP mv h' = SOME b ∧
+    EXISTS (λ(p,a). p) (MAP (λ(atoml,st_num,res). (is_match_row s_in st_num atoml mv,res)) tbl) ⇒
+    EXISTS (λ(p,a). p) (MAP (λ(atoml,st_num,res). (is_match_row s_in st_num atoml mv,res))
+                            (simp_tbl (mk_substitute_tbl tbl h' b)))
+Proof
+  Induct >-
+   gvs[mk_substitute_tbl_def, simp_tbl_def] >>
+  rpt strip_tac >>
+  simp[mk_substitute_tbl_def, simp_tbl_def] >>
+  gvs[] >|[
+  
+    PairCases_on ‘h’ >>
+    rename1 ‘(atoml, st_num, res)’ >>
+    gvs[MAP_MAP_o] >>
+    gvs[EXISTS_MAP] >>
+    imp_res_tac is_match_row_substitute_preserve1 >> gvs[]
+    ,
+    res_tac >>
+    gvs[mk_substitute_tbl_def, simp_tbl_def]
+  ]    
+QED
+
+
+Theorem exists_is_match_row_before_subst_simp:        
+  ∀ tbl s_in h' b mv.
+    ALOOKUP mv h' = SOME b ∧
+    EXISTS (λ(p,a). p) (MAP (λ(atoml,st_num,res). (is_match_row s_in st_num atoml mv,res))
+                            (simp_tbl (mk_substitute_tbl tbl h' b))) ⇒
+    EXISTS (λ(p,a). p) (MAP (λ(atoml,st_num,res). (is_match_row s_in st_num atoml mv,res)) tbl)
+Proof
+  Induct >-
+   gvs[mk_substitute_tbl_def, simp_tbl_def] >>
+  rpt strip_tac >>
+  gvs[mk_substitute_tbl_def, simp_tbl_def] >>
+  gvs[] >|[
+  
+    PairCases_on ‘h’ >>
+    rename1 ‘(atoml, st_num, res)’ >>
+    gvs[MAP_MAP_o] >>
+    gvs[EXISTS_MAP] >>
+    imp_res_tac is_match_row_substitute_preserve2 >> gvs[]
+    ,
+    res_tac >>
+    gvs[mk_substitute_tbl_def, simp_tbl_def]
+  ]    
+QED
+
+
+
+
+Theorem is_match_row_lists_subst_simp_eq:        
+∀tbl h' b mv s_in.
+       ALOOKUP mv h' = SOME b ⇒
+       MAP (λ(atoml,st_num,res). (is_match_row s_in st_num atoml mv,res))
+         (simp_tbl (mk_substitute_tbl tbl h' b)) =
+       MAP (λ(atoml,st_num,res). (is_match_row s_in st_num atoml mv,res)) tbl 
+Proof
+  Induct >>
+  rpt strip_tac >>
+  gvs[mk_substitute_tbl_def,simp_tbl_def] >>
+  PairCases_on ‘h’ >>
+  rename1 ‘(atoml, st_num, res)’ >>
+  gvs[MAP_MAP_o] >>
+  gvs[EXISTS_MAP] >>
+  
+  imp_res_tac is_match_row_substitute_preserve >>
+  gvs[]
+QED
+
+
+
+
+Theorem subst_simp_sem_tables_INDEX_FIND_congruence:
+  ∀ tbl mv s_in h' b i.
+    ALOOKUP mv h' = SOME b  ⇒
+    INDEX_FIND i (λ(p,a). p)
+               (MAP (λ(atoml,st_num,res). (is_match_row s_in st_num atoml mv,res)) (simp_tbl (mk_substitute_tbl tbl h' b))) =
+    INDEX_FIND i (λ(p,a). p)
+               (MAP (λ(atoml,st_num,res). (is_match_row s_in st_num atoml mv,res)) tbl)
+
+Proof
+  rpt strip_tac >>
+  imp_res_tac is_match_row_lists_subst_simp_eq >>
+  gvs[]
+QED
+
+
+
+Theorem subst_check_rows_sem_tables_INDEX_FIND_congruence:
+  ∀ tbl mv s_in h' b.
+    ALOOKUP mv h' = SOME b  ⇒
+    (check_all_rows_match s_in(simp_tbl (mk_substitute_tbl tbl h' b)) mv) =
+    (check_all_rows_match s_in tbl mv)
+Proof
+  gvs[check_all_rows_match_def] >>
+  rpt strip_tac >>
+  imp_res_tac is_match_row_lists_subst_simp_eq >>
+  gvs[]
+QED
+                      
+
+Theorem min_idx_till_subst_simp_invariant1:
+  ∀ tbl mv s_in h' b atoml st_num res .
+      ALOOKUP mv h' = SOME b  ⇒
+      min_idx_till (check_all_rows_match s_in (simp_tbl (mk_substitute_tbl ((atoml,st_num,res)::tbl) h' b)) mv) T =
+      min_idx_till (check_all_rows_match s_in ((atoml,st_num,res)::tbl) mv) T
+Proof
+  rpt strip_tac >> 
+  gvs[min_idx_till_def] >>
+  imp_res_tac subst_check_rows_sem_tables_INDEX_FIND_congruence >>
+  gvs[]  
+QED
+
+
+Theorem min_idx_till_subst_simp_invariant2:
+  ∀ tbl mv s_in h' b  .
+      ALOOKUP mv h' = SOME b  ⇒
+      min_idx_till (check_all_rows_match s_in (simp_tbl (mk_substitute_tbl (tbl) h' b)) mv) T =
+      min_idx_till (check_all_rows_match s_in (tbl) mv) T
+Proof
+  rpt strip_tac >> 
+  gvs[min_idx_till_def] >>
+  imp_res_tac subst_check_rows_sem_tables_INDEX_FIND_congruence >>
+  gvs[]  
+QED
+
+
+Theorem sem_tables_subst_simp_invariant:
+  ∀ tbl mv s_in h' b row .
+    ALOOKUP mv h' = SOME b   ⇒
+    sem_tables ([simp_tbl (mk_substitute_tbl (row::tbl) h' b)],s_in) mv =
+    sem_tables ([row::tbl],s_in) mv
+Proof
+  rpt strip_tac >>
+  PairCases_on ‘row’ >> rename1 ‘(atoml,st_num,res)’ >>
+  gvs[] >>
+        
+  simp[sem_tables_def, match_tbll_def] >>
+  gvs[match_tbl_def] >>
+  rpt (BasicProvers.FULL_CASE_TAC >> gvs[]) >>
+  
+  imp_res_tac min_idx_till_subst_simp_invariant1 >> gvs[] 
+QED
+  
+
+     
+Theorem prop1_var_single_tbl_verbose:
+  ∀ tbl mv h' b s_in.
+    ALOOKUP mv h' = SOME b ⇒
+    sem_tables (simp_tbll (mk_substitute_tbll [tbl] h' b),s_in) mv =
+    sem_tables ([tbl],s_in) mv
+Proof
+  Cases >-
+   (gvs[fv_tbll_def, mk_substitute_tbll_def, simp_tbll_def] >> 
+   gvs[fv_tbl_def, mk_substitute_tbl_def, simp_tbl_def]) >> 
+
+  rpt strip_tac >>
+  gvs[mk_substitute_tbll_def, simp_tbll_def] >> 
+  imp_res_tac sem_tables_subst_simp_invariant >>
+  gvs[]  
+QED
+            
+
+
+            
+Theorem prop1_var_tables_verbose:
+  ∀ tbls h b mv s_in.
+    ALOOKUP mv h = SOME b 
+    ⇒
+    sem_tables (simp_tbll (mk_substitute_tbll tbls h b),s_in) mv =
+    sem_tables (tbls,s_in) mv
+Proof
+
+  Induct_on ‘tbls’ >> rpt strip_tac >-
+   gvs[fv_tbll_def, mk_substitute_tbll_def, simp_tbll_def] >> 
+  rename1 ‘(tbl::tbll)’ >>
+
+  imp_res_tac prop1_var_single_tbl_verbose >>
+  first_x_assum (strip_assume_tac o (Q.SPECL [‘tbl’, ‘s_in’])) >>
+                
+  Cases_on ‘tbll’ >> gvs[] >> 
+  rename1 ‘(tbl::nexttbl::tbll)’ >>
+
+  gvs[sem_tables_def, match_tbll_def] >>
+  Cases_on ‘match_tbl tbl mv s_in’ >> gvs[] >>
+  rpt (BasicProvers.FULL_CASE_TAC >> gvs[]) >>
+
+  gvs[mk_substitute_tbll_def, simp_tbll_def] >>
+  gvs[match_tbll_def] >>     
+  Cases_on ‘match_tbl (simp_tbl (mk_substitute_tbl tbl h' b)) mv s_in’ >> gvs[] >>
+  rpt (BasicProvers.FULL_CASE_TAC >> gvs[]) >>
+
+  gvs[match_tbl_def] >>
+  rpt (BasicProvers.FULL_CASE_TAC >> gvs[]) >>
+  imp_res_tac min_idx_till_subst_simp_invariant2 >> gvs[]
+QED
+
+                          
+               
+Theorem prop1_var_tables:
+  prop1 table_structure
+Proof
+  rgs[prop1_def, table_structure_def, fv_in_p_def] >>
+
+  rpt strip_tac >>
+  Cases_on ‘p’ >>
+  rename1 ‘(tbls, s_in)’ >>
+
+  gvs[fv_tables_def, mk_substitute_tables_def, simp_tables_def] >>
+  imp_res_tac prop1_var_tables_verbose >> gvs[]    
+QED
+
+
         
            
 val _ = export_theory ();
